
\documentclass[letterpaper, reqno,11pt]{article}
\usepackage[margin=1.0in]{geometry}
\usepackage{color,latexsym,amsmath,amssymb}
\usepackage{fancyhdr}
\usepackage{amsthm}
\usepackage{graphicx}

\newdimen\R
\R=0.8cm
\pagestyle{fancy}
\lhead{Analysis of Algorithms Exercises 1}
\rhead{Yuchong Pan}
\begin{document}
\pagenumbering{arabic}
\title{Analysis of Algorithms Exercises 1}
\author{Yuchong Pan}
\date{\today}
\newtheorem{thm}{Theorem}[section]
\newtheorem{lemma}{Lemma}[section]
\newtheorem{defn}{Definition}[section]
\maketitle
%

\noindent {\bf Exercise 1.14} Multiply by $N$:
\begin{equation*}
    NA_N=N+2\sum_{1\leq j\leq N}A_{j-1}\quad{\rm for}\ N>0.
\end{equation*}
Subtract the same formula for $N-1$ to eliminate the sum:
\begin{equation*}
    NA_N-(N-1)A_{N-1}=1+2A_{N-1}\quad{\rm for}\ N>1.
\end{equation*}
Then rearrange terms to get a simple recurrence
\begin{equation*}
    NA_N=(N+1)A_{N-1}+1\quad{\rm for}\ N>1.
\end{equation*}
This can be solved by dividing both sides by $N(N+1)$:
\begin{equation*}
    \frac{A_N}{N+1}=\frac{A_{N-1}}{N}+\frac{1}{N(N+1)}\quad{\rm for}\ N>1.
\end{equation*}
Iterating, we are left with the sum
\begin{equation*}
    \frac{A_N}{N+1}=\frac{A_1}{2}+\sum_{2\leq i\leq N}\frac{1}{N(N+1)}\quad{\rm for}\ N>1.
\end{equation*}
Since $A_1=1$, then
\begin{equation*}
    \frac{A_N}{N+1}=\frac{1}{2}+\sum_{2\leq i\leq N}\frac{1}{N(N+1)}=\frac{N}{N+1}\quad{\rm for}\ N>1.
\end{equation*}
Hence,
\begin{equation*}
    A_N=N\quad{\rm for}\ N>0.
\end{equation*}

\end{document}
